Runwai/Gadget/Func.lean
@@ -62,8 +62,8 @@ lemma isZero_eval_eq_branch_semantics {x y inv: Expr} {σ: Env.ValEnv} {T: Env.T
 
 lemma isZero_typing_soundness (Δ: Env.ChipEnv) (Η: Env.UsedNames) (Γ: Env.TyEnv) (φ₁ φ₂ φ₃: Ast.Predicate)
   (x y inv u₁ u₂: String)
-  (htx: Env.lookupTy Γ x = (Ty.refin Ast.Ty.field φ₁))
-  (hty: Env.lookupTy Γ y = (Ty.refin Ast.Ty.field φ₂))
+  (htx: Env.getTy Γ x = (Ty.refin Ast.Ty.field φ₁))
+  (hty: Env.getTy Γ y = (Ty.refin Ast.Ty.field φ₂))
   (htinv: @Ty.TypeJudgment Δ Γ Η (.var inv) (Ty.refin Ast.Ty.field φ₃))
   (hne₁: ¬ x = u₁)
   (hne₂: ¬ y = u₁)
@@ -72,15 +72,15 @@ lemma isZero_typing_soundness (Δ: Env.ChipEnv) (Η: Env.UsedNames) (Γ: Env.TyE
     (Ast.Expr.letIn u₁ (.assertE (.var y) (.fieldExpr (.fieldExpr (.fieldExpr (.constF 0) .sub (.var x)) .mul (.var inv)) (.add) (.constF 1)))
       (Ast.Expr.letIn u₂ (.assertE (.fieldExpr (.var x) .mul (.var y)) (.constF 0)) (.var u₂)))
     (Ty.refin Ast.Ty.unit (Ast.Predicate.ind (exprEq (.var y) (.branch (.binRel (.var x) (.eq) (.constF 0)) (.constF 1) (.constF 0))))) := by {
-    apply Ty.TypeJudgment.TE_LetIn; apply lookup_update_self;
+    apply Ty.TypeJudgment.TE_LetIn; apply get_update_self;
     apply Ty.TypeJudgment.TE_Assert; apply Ty.TypeJudgment.TE_VarEnv; exact hty
     repeat apply Ty.TypeJudgment.TE_BinOpField
     apply Ty.TypeJudgment.TE_ConstF; apply Ty.TypeJudgment.TE_VarEnv; exact htx; exact htinv
-    apply Ty.TypeJudgment.TE_ConstF; apply Ty.TypeJudgment.TE_LetIn; apply lookup_update_self
+    apply Ty.TypeJudgment.TE_ConstF; apply Ty.TypeJudgment.TE_LetIn; apply get_update_self
     apply Ty.TypeJudgment.TE_Assert; apply Ty.TypeJudgment.TE_BinOpField; apply Ty.TypeJudgment.TE_VarEnv
-    rw[← htx]; apply lookup_update_ne; exact hne₁
+    rw[← htx]; apply get_update_ne; exact hne₁
     apply Ty.TypeJudgment.TE_VarEnv
-    rw[← hty]; apply lookup_update_ne; exact hne₂
+    rw[← hty]; apply get_update_ne; exact hne₂
     apply Ty.TypeJudgment.TE_ConstF
     have h_sub : @Ty.SubtypeJudgment Δ (Env.updateTy
       (Env.updateTy Γ u₁
@@ -104,10 +104,10 @@ lemma isZero_typing_soundness (Δ: Env.ChipEnv) (Η: Env.UsedNames) (Γ: Env.TyE
               (Expr.constF 1))))
         set φ₂ := (Ast.Predicate.ind (exprEq ((Expr.var x).fieldExpr FieldOp.mul (Expr.var y)) (Expr.constF 0)))
         have h₃ := h₂ u₁ (Ty.unit.refin φ₁)
-        have h₄: Env.lookupTy (Env.updateTy (Env.updateTy Γ u₁ (Ty.unit.refin φ₁)) u₂ (Ty.unit.refin φ₂)) u₁ = (Ty.unit.refin φ₁) := by {
-          apply lookup_update_ne_of_lookup
+        have h₄: Env.getTy (Env.updateTy (Env.updateTy Γ u₁ (Ty.unit.refin φ₁)) u₂ (Ty.unit.refin φ₂)) u₁ = (Ty.unit.refin φ₁) := by {
+          apply get_update_ne_of_get
           exact hne₃
-          apply lookup_update_self
+          apply get_update_self
         }
         have h₅ := h₃ h₄
         rw[h₄] at h₅
@@ -119,7 +119,7 @@ lemma isZero_typing_soundness (Δ: Env.ChipEnv) (Η: Env.UsedNames) (Γ: Env.TyE
       }
     apply Ty.TypeJudgment.TE_SUB
     apply Ty.TypeJudgment.TE_VarEnv
-    apply lookup_update_self
+    apply get_update_self
     exact h_sub
 }
 
@@ -131,18 +131,18 @@ lemma iszero_func_typing_soundness (Δ: Env.ChipEnv) (Η: Env.UsedNames) (Γ: En
       (Ty.refin Ast.Ty.unit (Ast.Predicate.ind (exprEq (.var "y") (.branch (.binRel (.var "x") (.eq) (.constF 0)) (.constF 1) (.constF 0)))))))) := by {
       repeat
         apply Ty.TypeJudgment.TE_Abs
-        apply lookup_update_self
+        apply get_update_self
       apply isZero_typing_soundness
-      apply lookup_update_ne_of_lookup
+      apply get_update_ne_of_get
       simp
-      apply lookup_update_ne_of_lookup
+      apply get_update_ne_of_get
       simp
-      apply lookup_update_self
-      apply lookup_update_ne_of_lookup
+      apply get_update_self
+      apply get_update_ne_of_get
       simp
-      apply lookup_update_self
+      apply get_update_self
       apply Ty.TypeJudgment.TE_VarEnv
-      apply lookup_update_self
+      apply get_update_self
       repeat simp
     }
 
@@ -191,48 +191,48 @@ abbrev koalabear_word_range_checker_func: Ast.Expr :=
         (.var "u₁₁"))))))))))))))))))))))))))))))))))))))
 
 lemma koalabear_word_range_checker_subtype_soundness {Γ Δ}
-  (hb₁: Env.lookupTy Γ "b₀" = some (bit_value_type "most_sig_byte_decomp_0"))
-  (hb₂ : Env.lookupTy Γ "b₁" = some (bit_value_type "most_sig_byte_decomp_1"))
-  (hb₃: Env.lookupTy Γ "b₂" = some (bit_value_type "most_sig_byte_decomp_2"))
-  (hb₄ : Env.lookupTy Γ "b₃" = some (bit_value_type "most_sig_byte_decomp_3"))
-  (hb₅: Env.lookupTy Γ "b₄" = some (bit_value_type "most_sig_byte_decomp_4"))
-  (hb₆ : Env.lookupTy Γ "b₅" = some (bit_value_type "most_sig_byte_decomp_5"))
-  (hb₇: Env.lookupTy Γ "b₆" = some (bit_value_type "most_sig_byte_decomp_6"))
-  (hb₈ : Env.lookupTy Γ "b₇" = some (bit_value_type "most_sig_byte_decomp_7"))
-  (hu₁: Env.lookupTy Γ "u₁" = some (Ast.Ty.unit.refin
+  (hb₁: Env.getTy Γ "b₀" = some (bit_value_type "most_sig_byte_decomp_0"))
+  (hb₂ : Env.getTy Γ "b₁" = some (bit_value_type "most_sig_byte_decomp_1"))
+  (hb₃: Env.getTy Γ "b₂" = some (bit_value_type "most_sig_byte_decomp_2"))
+  (hb₄ : Env.getTy Γ "b₃" = some (bit_value_type "most_sig_byte_decomp_3"))
+  (hb₅: Env.getTy Γ "b₄" = some (bit_value_type "most_sig_byte_decomp_4"))
+  (hb₆ : Env.getTy Γ "b₅" = some (bit_value_type "most_sig_byte_decomp_5"))
+  (hb₇: Env.getTy Γ "b₆" = some (bit_value_type "most_sig_byte_decomp_6"))
+  (hb₈ : Env.getTy Γ "b₇" = some (bit_value_type "most_sig_byte_decomp_7"))
+  (hu₁: Env.getTy Γ "u₁" = some (Ast.Ty.unit.refin
                                   (Ast.Predicate.ind
                                     (Ast.exprEq
                                       (bits_to_byte_expr "most_sig_byte_decomp_0" "most_sig_byte_decomp_1" "most_sig_byte_decomp_2" "most_sig_byte_decomp_3"
                                                         "most_sig_byte_decomp_4" "most_sig_byte_decomp_5" "most_sig_byte_decomp_6" "most_sig_byte_decomp_7")
                                       (Ast.Expr.var "value_3")))))
-  (hu₂: Env.lookupTy Γ "u₂" = some                               (Ast.Ty.unit.refin
+  (hu₂: Env.getTy Γ "u₂" = some                               (Ast.Ty.unit.refin
                                 (Ast.Predicate.ind
                                   (Ast.exprEq (Ast.Expr.var "most_sig_byte_decomp_7") (Ast.Expr.constF 0)))))
-  (hu₃: Env.lookupTy Γ "u₃" = some (eq_mul_refinement "and_most_sig_byte_decomp_0_to_2" "most_sig_byte_decomp_0" "most_sig_byte_decomp_1"))
-  (hu₄: Env.lookupTy Γ "u₄" = some (eq_mul_refinement "and_most_sig_byte_decomp_0_to_3" "and_most_sig_byte_decomp_0_to_2" "most_sig_byte_decomp_2"))
-  (hu₅: Env.lookupTy Γ "u₅" = some (eq_mul_refinement "and_most_sig_byte_decomp_0_to_4" "and_most_sig_byte_decomp_0_to_3" "most_sig_byte_decomp_3"))
-  (hu₆: Env.lookupTy Γ "u₆" = some (eq_mul_refinement "and_most_sig_byte_decomp_0_to_5" "and_most_sig_byte_decomp_0_to_4" "most_sig_byte_decomp_4"))
-  (hu₇: Env.lookupTy Γ "u₇" = some (eq_mul_refinement "and_most_sig_byte_decomp_0_to_6" "and_most_sig_byte_decomp_0_to_5" "most_sig_byte_decomp_5"))
-  (hu₈: Env.lookupTy Γ "u₈" = some (eq_mul_refinement "and_most_sig_byte_decomp_0_to_7" "and_most_sig_byte_decomp_0_to_6" "most_sig_byte_decomp_6"))
-  (hu₉: Env.lookupTy Γ "u₉" = some                           (Ast.Ty.unit.refin
+  (hu₃: Env.getTy Γ "u₃" = some (eq_mul_refinement "and_most_sig_byte_decomp_0_to_2" "most_sig_byte_decomp_0" "most_sig_byte_decomp_1"))
+  (hu₄: Env.getTy Γ "u₄" = some (eq_mul_refinement "and_most_sig_byte_decomp_0_to_3" "and_most_sig_byte_decomp_0_to_2" "most_sig_byte_decomp_2"))
+  (hu₅: Env.getTy Γ "u₅" = some (eq_mul_refinement "and_most_sig_byte_decomp_0_to_4" "and_most_sig_byte_decomp_0_to_3" "most_sig_byte_decomp_3"))
+  (hu₆: Env.getTy Γ "u₆" = some (eq_mul_refinement "and_most_sig_byte_decomp_0_to_5" "and_most_sig_byte_decomp_0_to_4" "most_sig_byte_decomp_4"))
+  (hu₇: Env.getTy Γ "u₇" = some (eq_mul_refinement "and_most_sig_byte_decomp_0_to_6" "and_most_sig_byte_decomp_0_to_5" "most_sig_byte_decomp_5"))
+  (hu₈: Env.getTy Γ "u₈" = some (eq_mul_refinement "and_most_sig_byte_decomp_0_to_7" "and_most_sig_byte_decomp_0_to_6" "most_sig_byte_decomp_6"))
+  (hu₉: Env.getTy Γ "u₉" = some                           (Ast.Ty.unit.refin
                   (Ast.Predicate.ind
                     (Ast.exprEq (Ast.Expr.constF 0)
                       ((Ast.Expr.var "and_most_sig_byte_decomp_0_to_7").fieldExpr Ast.FieldOp.mul
                         (Ast.Expr.var "value_0"))))))
-  (hu₁₀: Env.lookupTy Γ "u₁₀" = some                           (Ast.Ty.unit.refin
+  (hu₁₀: Env.getTy Γ "u₁₀" = some                           (Ast.Ty.unit.refin
                 (Ast.Predicate.ind
                   (Ast.exprEq (Ast.Expr.constF 0)
                     ((Ast.Expr.var "and_most_sig_byte_decomp_0_to_7").fieldExpr Ast.FieldOp.mul
                       (Ast.Expr.var "value_1"))))))
-  (hu₁₁: Env.lookupTy Γ "u₁₁" = some                           (Ast.Ty.unit.refin
+  (hu₁₁: Env.getTy Γ "u₁₁" = some                           (Ast.Ty.unit.refin
                 (Ast.Predicate.ind
                   (Ast.exprEq (Ast.Expr.constF 0)
                     ((Ast.Expr.var "and_most_sig_byte_decomp_0_to_7").fieldExpr Ast.FieldOp.mul
                       (Ast.Expr.var "value_2"))))))
-  ( hl₀: Env.lookupTy Γ "value_0" = some (field_lt_const 256))
-  ( hl₁: Env.lookupTy Γ "value_1" = some (field_lt_const 256))
-  ( hl₂: Env.lookupTy Γ "value_2" = some (field_lt_const 256))
-  ( hl₃: Env.lookupTy Γ "value_3" = some (field_lt_const 256))
+  ( hl₀: Env.getTy Γ "value_0" = some (field_lt_const 256))
+  ( hl₁: Env.getTy Γ "value_1" = some (field_lt_const 256))
+  ( hl₂: Env.getTy Γ "value_2" = some (field_lt_const 256))
+  ( hl₃: Env.getTy Γ "value_3" = some (field_lt_const 256))
   : @Ty.SubtypeJudgment Δ Γ
       (Ty.unit.refin (Predicate.ind (exprEq (Expr.constF 0) ((Expr.var "and_most_sig_byte_decomp_0_to_7").fieldExpr FieldOp.mul (Expr.var "value_2")))))
       (Ast.Ty.refin Ast.Ty.unit (Ast.Predicate.ind
@@ -482,79 +482,79 @@ lemma koalabear_word_range_checker_func_typing_soundness (Δ: Env.ChipEnv) (Η: 
         .lt (.constZ 2130706433)))))))))))))))))))))) := by {
   repeat
     apply Ty.TypeJudgment.TE_Abs
-    apply lookup_update_self
+    apply get_update_self
   repeat
     apply Ty.TypeJudgment.TE_LetIn;
-    apply lookup_update_self;
+    apply get_update_self;
     apply Ty.TypeJudgment.TE_Assert
     apply Ty.TypeJudgment.TE_BinOpField
     apply Ty.TypeJudgment.TE_VarEnv
-    apply lookup_update_ne
+    apply get_update_ne
     simp
     apply Ty.TypeJudgment.TE_BinOpField
     apply Ty.TypeJudgment.TE_VarEnv
-    apply lookup_update_ne
+    apply get_update_ne
     simp
     repeat apply Ty.TypeJudgment.TE_ConstF
 
   apply Ty.TypeJudgment.TE_LetIn;
-  apply lookup_update_self;
+  apply get_update_self;
   apply Ty.TypeJudgment.TE_Assert
   repeat apply Ty.TypeJudgment.TE_BinOpField
   apply Ty.TypeJudgment.TE_VarEnv
-  apply lookup_update_ne
+  apply get_update_ne
   simp
   repeat
     apply Ty.TypeJudgment.TE_BinOpField
     apply Ty.TypeJudgment.TE_VarEnv
-    apply lookup_update_ne
+    apply get_update_ne
     simp
     repeat apply Ty.TypeJudgment.TE_ConstF
   apply Ty.TypeJudgment.TE_VarEnv
-  apply lookup_update_ne
+  apply get_update_ne
   simp
 
   apply Ty.TypeJudgment.TE_LetIn;
-  apply lookup_update_self;
+  apply get_update_self;
   apply Ty.TypeJudgment.TE_Assert
   apply Ty.TypeJudgment.TE_VarEnv
-  apply lookup_update_ne
+  apply get_update_ne
   simp
   apply Ty.TypeJudgment.TE_ConstF
 
   repeat
     apply Ty.TypeJudgment.TE_LetIn;
-    apply lookup_update_self;
+    apply get_update_self;
     apply Ty.TypeJudgment.TE_Assert
     apply Ty.TypeJudgment.TE_VarEnv
-    apply lookup_update_ne
+    apply get_update_ne
     simp
     apply Ty.TypeJudgment.TE_BinOpField
     repeat
       apply Ty.TypeJudgment.TE_VarEnv
-      apply lookup_update_ne
+      apply get_update_ne
       simp
 
   repeat
     apply Ty.TypeJudgment.TE_LetIn;
-    apply lookup_update_self;
+    apply get_update_self;
     apply Ty.TypeJudgment.TE_Assert
     apply Ty.TypeJudgment.TE_ConstF
     apply Ty.TypeJudgment.TE_BinOpField
     repeat
       apply Ty.TypeJudgment.TE_VarEnv
-      apply lookup_update_ne
+      apply get_update_ne
       simp
 
   apply Ty.TypeJudgment.TE_SUB
   apply Ty.TypeJudgment.TE_VarEnv
-  apply lookup_update_self
+  apply get_update_self
   apply koalabear_word_range_checker_subtype_soundness
   repeat
-    apply lookup_update_ne
+    apply get_update_ne
     simp
-  apply lookup_update_self
+  apply get_update_self
   repeat
-    apply lookup_update_ne
+    apply get_update_ne
     simp
 }
