Runwai/Tactic.lean
@@ -6,15 +6,15 @@ macro_rules
 | `(tactic| auto_trace_index) => `(tactic|
     repeat
       apply Ty.TypeJudgment.TE_LetIn
-      · apply lookup_update_self
+      · apply get_update_self
       · apply Ty.TypeJudgment.TE_ArrayIndex
         apply Ty.TypeJudgment.TE_ArrayIndex
         apply Ty.TypeJudgment.TE_VarEnv
-        apply lookup_update_ne
+        apply get_update_ne
         try (simp)
         apply Ty.TypeJudgment.TE_VarEnv
-        try (apply lookup_update_self)
-        try (apply lookup_update_ne)
+        try (apply get_update_self)
+        try (apply get_update_ne)
         try (simp)
         apply constZ_refine_lt
         try (simp)
@@ -24,7 +24,7 @@ syntax "auto_let_assert" : tactic
 macro_rules
 | `(tactic| auto_let_assert) => `(tactic|
     apply Ty.TypeJudgment.TE_LetIn;
-    apply lookup_update_self;
+    apply get_update_self;
     apply Ty.TypeJudgment.TE_Assert;
   )
 
@@ -32,12 +32,12 @@ syntax "auto_resolve_varenv" : tactic
 macro_rules
 | `(tactic| auto_resolve_varenv) => `(tactic|
     apply Ty.TypeJudgment.TE_VarEnv;
-    apply lookup_update_ne;
+    apply get_update_ne;
     simp;
   )
 
 /-
     apply Ty.TypeJudgment.TE_VarEnv
-    apply lookup_update_ne
+    apply get_update_ne
     simp
 -/
